src/lib/GPU.Array.fsti
@@ -183,17 +183,16 @@ val gpu_array_unslice_1_underspec
     (bigstar 0 sz (gpu_pts_to_array1 arr #f))
     (fun _ -> exists* v. gpu_pts_to_array arr #f v)
 
-```pulse
-ghost val fn gpu_slice_concat
-  (#a:Type0)
+val gpu_slice_concat
+  (#a:Type u#0)
   (#sz:nat)
   (arr : gpu_array a sz)
   (#[exact (`1.0R)] f : perm)
   (#s1 #s2: erased (seq a))
   (i n m:nat)
-  requires gpu_pts_to_array_slice #a #sz arr #f i n s1 ** gpu_pts_to_array_slice #a #sz arr #f n m s2
-  ensures  gpu_pts_to_array_slice #a #sz arr #f i m (Seq.Base.append s1 s2)
-```
+  : stt_ghost unit emp_inames
+      (gpu_pts_to_array_slice arr #f i n s1 ** gpu_pts_to_array_slice arr #f n m s2)
+      (fun _ -> gpu_pts_to_array_slice arr #f i m (Seq.Base.append s1 s2))
 
 // ```xx
 // fn memcpy_host_to_device
