src/lib/GPU.SizeT.fsti
@@ -17,12 +17,12 @@ let fits_sizet (x:nat)
   = assert_norm (pow2 64 == 0x10000000000000000);
     FStar.SizeT.fits_u64_implies_fits x
 
-[@@coercion] unfold let sizet_to_int  (x: SZ.t)  : GTot int = SZ.v x
-[@@coercion] unfold let u32_to_int    (x: U32.t) : GTot int = U32.v x
-[@@coercion] unfold let u64_to_int    (x: U64.t) : GTot int = U64.v x
-[@@coercion] unfold let sizet_to_eint (x: SZ.t)  : erased int = SZ.v x
-[@@coercion] unfold let u32_to_eint   (x: U32.t) : erased int = U32.v x
-[@@coercion] unfold let u64_to_eint   (x: U64.t) : erased int = U64.v x
+[@@coercion; Pulse.Lib.Core.pulse_unfold] unfold let sizet_to_int  (x: SZ.t)  : GTot int = SZ.v x
+[@@coercion; Pulse.Lib.Core.pulse_unfold] unfold let u32_to_int    (x: U32.t) : GTot int = U32.v x
+[@@coercion; Pulse.Lib.Core.pulse_unfold] unfold let u64_to_int    (x: U64.t) : GTot int = U64.v x
+[@@coercion; Pulse.Lib.Core.pulse_unfold] unfold let sizet_to_eint (x: SZ.t)  : erased int = SZ.v x
+[@@coercion; Pulse.Lib.Core.pulse_unfold] unfold let u32_to_eint   (x: U32.t) : erased int = U32.v x
+[@@coercion; Pulse.Lib.Core.pulse_unfold] unfold let u64_to_eint   (x: U64.t) : erased int = U64.v x
 
 (* assumption, add to F*? *)
 val sizet_to_u32 (x: SZ.t) 
